_out/html/html-single/-verso-search/searchIndex_81.js
@@ -1,1 +1,1 @@
-window.docContents[81].resolve({"/#PSBP-Documentation--The--PSBP--Library-type-classes":{"id":"/#PSBP-Documentation--The--PSBP--Library-type-classes","header":"3. The  PSBP  Library type classes","context":"PSBP Documentation","contents":"\n\n\n\n\n\n\n\n\n\n\n\n\n\n"}});
+window.docContents[81].resolve({"/#PSBP-Documentation--The--PSBP--Library-type-classes":{"id":"/#PSBP-Documentation--The--PSBP--Library-type-classes","header":"4. The  PSBP  Library type classes","context":"PSBP Documentation","contents":"\n\n\n\n\n\n\n\n\n\n\n\n\n\n"}});
