PsbpDocumentation/PsbpDocumentation.lean
@@ -1,4 +1,5 @@
 import VersoManual
+
 import PsbpDocumentation.Meta.Lean
 
 open Verso.Genre Manual
@@ -15,59 +16,389 @@ set_option pp.rawOnError true
 authors := ["Luc Duponcheel"]
 %%%
 
-# Warning
+# About
 
-This is work in progress.
+This document is about the
+[`Lean` `PSBP` library](https://github.com/LucDuponcheelAtGitHub/PSBP),
+in what follows, also simply called `PSBP`.
 
-The book and it's code is far from complete and may change.
+This document can be seen as a, somewhat special, not to say opinionated, programming course, especiallty useful for
+mathematicians and/or computer scientists, researchers as well as students, possible future researchers, who are
+interested in mathematical foundations of programming.
 
-For now I do not use the universe capabilities of `Lean`.
+The code of this document can be seen as a programming course for `Lean` itself. `Lean` turns out to be both a very
+demanding and very helpful student.
 
-I (try to) format code is a consistent way.
+When I worked with Doatse Swierstra at the University of Utrecht, he once told me that, apart from sound proving
+techniques like "proof by induction", there is also this unsound proving technique "proof by intimidation". When no
+student complains about the correctness of a proof, the proof is correct. Of course, Doaitse did not apply this
+technique when teaching. `Lean` would be this very demanding student asking you for more and more into proof details
+before accepting the correctness of the proof. But `Lean` would also be this very helpful student that would be able to
+infer the proof details for you if you are stuck.
 
-# Introduction
+The first sections of this course do not always explain all concepts that they deal with. Please keep on reading. All
+concepts will, eventually, be explained. Starting from section "The PSBP Library type classes" the course is self
+contained and requires, at least in theory, no previous knowledge.
 
-Lean defines type classes `Functor`, `Applicative` and `Monad`. They specify computation capabilities. Think of
-computations as effectful expressions. They are operational artifacts. They do not really have a meaning in the
-mathematical sense. Functions, on the other hand, are denotational artifacts. They do have a meaning in the mathematical
-sense.
+So let's end this section with a, somewhat offensive, motivation to keep on reading this document.
 
-This document refers to effectful function as programs. So how to specify program capabilities? That is what the `PSBP`
-library is all about. `PSPB` stands for "Program Specification Based Programming". `PSBP` is a library that allows you
-to write program specifications in terms of program capabilities that are specified using type classes. You can then
-materialize those program specifications according to instances of the type classes in terms of which the program
-specifications are written. `PSBP` can be seen as a library level programming language. In what follows we will, by
-abuse of language, often write "program" instead of "program specification" or
-"program (specification) materialization". Hopefully this will not lead to confusion.
+If `Lean` can understand the course then you should be able to understand it as well.
 
-Just like expressions are evaluated to yield a result value, computations are executed to a result value, but, executing
-them may also perform side effects along the way. Just like functions, programs, by running them, transform initial
-(argument) values to filan (result) values, but, they may perform side effects along the way.
+# Naming conventions
 
-Why programming in terms of program specifications instead of in terms of computations? Both programs and computations
-form a component system. The difference is that programs are closed components, while computations are open components.
-Programming with programs is pointfree programming while programming with computations is pointful programming.
+In this document, `program`, intentionally written in typewriter font, has a specific, technical meaning while the word
+programming has a general meaning. For general purposes, this document uses the word code instead of the word program.
+As a consequence, in this document, the word programming means (the process of) writing code.
 
-In my opinion, it is a more elegant to program pointfree than to program pointful. Likewise, in my opinion, it is more
-elegant to reason in terms of pointffree laws than to reason in terms of with pointful laws. Of course, this is all a
-matter of taste. I hope to convince you that pointfree is more elegant than pointful.
+I hope that this naming convention does not lead to any confusion.
 
-By the way, it is alse possible, and sometimes necessary, to program positional using `PSBP`. Positional programming is
-similar to pointful programming. It is is useful for writing recipe-like programs, where, starting from an initial
-value, intermediate values are constructed, and. together with the initial value, are passed to the next step, until a
-final value is produced. The initial value and intermediate values are accessed positionally. More about this later.
+`PSBP` stands for "Program Specification Based Programming" (using the naming conventions above).
 
-By the way, a value can be a single-value or a multi-value, repesented a (nested) tuple. More about this later.
+`PSBP` is a pointfree effectful functional programming library, written using the `Lean` programming language.
 
-# The `PSBP` Library type classes
+In what follows `Lean` will rarely explictly be mentioned. It will implicitly be taken for granted.
+
+`PSBP` can be seen as a programming DSL, a Domain Specific Language for the programming domain.
+
+`PSBP` has a variety of programming related binary type constructor classes, among others `Functional`, `Functorial`,
+`Creational`, `Sequential` and `Conditional`. `PSBP` code consistently names their binary type constructor parameter
+`program`.
+
+The `PSPB` type constructor classes, just like all other classes, are specifications, also called interfaces in the
+programming world. They have members that declare basic program specifications and basic program specification
+combinators to combine program specifications to composite program specifications. Derived program specifications and
+derived program specification combinators can then be defined in terms of (declared or defined) program specifications
+and (declared or defined) program specification combinators. As such program specifications are components of a
+component system.
+
+The `Lean` standard library has a variety of computing related unary type constructor classes, among others `Functor`,
+`Applicative` and `Monad`. `PSBP` code consistently names their unary type constructor parameter `computation`.
+
+The `Lean` standard library type constructor classes above, just like all other classes, are specifications, also called
+interfaces in the programming world. They have members that declare basic computation specifications and basic
+computation specification combinators to combine computation specifications to composite computation specifications.
+Derived computation specifications and derived computation specification combinators can then be defined in terms of
+(declared or defined) computation specifications and (declared or defined) computation specification combinators. As
+such computation specifications are components of a component system.
+
+By now you may be asking why I used program specification resp. computation specification instead of simply using
+program resp. computation. First of all, because program specifications resp. computation specifications are
+specifications. Type constructor class instances, also called implemenations in the programming world, of the various
+type constructor classes, in terms of whose members program specifications resp. computation specifications are defined,
+need to be given to materialize program specifications resp. computation specifications. It are those materializations
+that are called programs resp. computations.
+
+In what follows, by abuse of language, I will often also use the word program (recall, a materialization of a program
+specification corresponding to instances of programming related type constructor classes) instead of program
+specification and often also use the word computation (recall, a materialization of a computation specification
+corresponding to instances of computing related type constructor classes) instead of computation specification.
+
+Hopefully this abuse of language does not lead to any confusion.
+
+It is instructive to compare this abuse of language with the title
+[Ceci n'est pas une pipe](https://en.wikipedia.org/wiki/The_Treachery_of_Images)
+of the painting of René Magritte. The painting itself is, of course, not a pipe, it is a description of a pipe.
+Yet, when you look at the painting, you might think of it as being a pipe. Much in the same way, when an architect is
+showing you the specification of a house, for example as a 3D animation (a special kind of description), communication,
+by abuse of language, happens using words like kitchen resp. bathroom instead of kitchen specification resp. bathroom
+specification.
+
+# Programs versus Computations
+
+The standard `Lean` library already enables Computation Specification Based Programming.
+
+So why promoting Program Specification Based Programming in the first place?
+
+In short, informally, it is all a matter of taste
+(you may wish to give up reading this document).
+
+In short, formally, because of progressive insight into what programming, writing code, is all about.
+
+Let's explain this in terms of the history about my progressive insight
+(you may wish to ignore what follows, not being interested in my personal history).
+
+I am a retired mathematician.
+
+Mathematics is generally agreed upon to be useful to understand the reality we are all part of. For example to
+understand problem domains some of us are, professionaly, confronted with.
+
+Bridge building engineers may benefit form studying appropriate mathematics to understand what bridges are all about.
+Vehicle building engineers may benefit form studying appropriate mathematics to understand what vehicles are all about.
+Likewise, programming engineers (programmers) may benefit form studying appropriate mathematics to understand what
+programs are all about.
+
+Separating specifications from implementations is generally agreed upon to be useful to understand problem domains.
+
+A bridge specification states, for example, that it must be able to carry the weight of a number of vehicles. How it is
+able to carry that weight is an implementation concern. Maybe one bridge is more pleasing to look at as another one. A
+vehicle specification states, for example, that it must be able to transport a number of passengers. How it is able to
+transport that number of passengers is an implementation concern. Maybe one car is more comfortable than another one. A
+program specification states, for example, that a program must be able to create composite data and to perform
+conditional logic. How it is able to create composite data and to perform conditional logic is an implementation
+concern. Maybe one program is more CPU (or GPU or NPU) effecient, or less RAM consuming than another one.
+
+Note that I wrote bridge, resp. car, resp. program as an abbreviation of materialization corresponding to an implementation
+of the bridge specification, resp. materialization corresponding to an implementation of the car specification, resp.
+materialization corresponding to an implementation of the program specification.
+
+I have always been interested in mathematics, so I followed the typical mathematics oriented education path from
+secondary school all the way to obtaining a PhD in mathematics. Now I realize that obtaining a PhD (in mathematics) is
+just a beginning. It shows that you are able to use 20% imagination and 80% transpiration to be creative in a particular
+area (of mathematics).
+
+I did, among others, mathematics research on
+[Non-archimedean induced representations of compact zerodimensional groups](https://www.numdam.org/article/CM_1986__57_1_3_0.pdf).
+Not that it matters much for the content of this document. What does matter is that I soon realized that, those days, in
+Belgium, mathematics could mainly be done as a backyard ritual, so, in order to earn money for a living, I decided to
+become a programmer. being adicted to mathematics research, I also decided to do computer science research as a late at
+night hobby (typically starting at 9PM).
+
+I studied function level programming systems, supported by the pointfree, effectfree functional programming language
+[`FP`](https://en.wikipedia.org/wiki/FP_%28programming_language%29).
+
+I published a paper
+[Acceptable functional programming systems](https://link.springer.com/article/10.1007/BF00268076)
+about a pointfree effectfree functional programming library. I wrote the paper together with my twin brother Marc, who
+is also a mathematician. The library was written using the
+[`Pascal`](https://en.wikipedia.org/wiki/Pascal_%28programming_language%29) programming language.
+
+The first functional programming language I used extensively was
+[`Miranda`](https://www.cs.kent.ac.uk/people/staff/dat/Miranda/).
+`Miranda` turned out to be a perfect language to learn (not to say become addicted to) functional programming.
+
+The next functional programming language I used extensively was `Gofer`, later evolving to
+[`Hugs`](https://www.haskell.org/Hugs/).
+`Gofer` was the first functional programming language supporting type constructor classes. They are appropriate to write
+the computing related specifications of effectful pointful functional programming libraries. The mathematical
+foundations of those specifications are [monads](https://en.wikipedia.org/wiki/Monad_%28functional_programming%29).
+
+I published the following papers
+
+1. [Composing monads](https://web.cecs.pdx.edu/~mpj/pubs/RR-1004.pdf),
+2. [On the expressive power of constructor classes](https://link.springer.com/chapter/10.1007/978-1-4471-3573-9_3),
+3. [Deterministic crror-correcting combinator parsers](https://www.cs.tufts.edu/~nr/cs257/archive/doaitse-swierstra/error-correcting.pdf), and
+4. [Using catamorphisms, subtypes and monad transformers for writing modular functional interpeters](https://citeseerx.ist.psu.edu/document?repid=rep1&type=pdf&doi=1cdebf7b88435a38156f62df1a7189b6d8ca3fe3).
+
+The first paper was written, as a late night hobby, together with Mark P. Jones, the author of `Gofer`. What is
+special about that paper is that we had never physically met each other. Those were the early days of the internet. We
+wrote the paper (and the code that came with it) together by sending emails with attachments to each other. In fact, it
+turned out to be an efficient way to work together. While one of us was sleeping (in Europe resp. the USA) the other one
+was working (in the USA resp. Europe). The paper also contained some equational proofs. Those days, they were simply
+encoded as lists of expressions representing equational proof steps. `Gofer` did not have a formal proof correctness
+reviewing mechanism like Lean has, but, type correctness provided at least some formal proof correctness confidence.
+
+The other papers were written when I was working, for two years, at the University of Utrecht. That was a unique
+experience for me for which I am, forever, greatful to Doaitse Swierstrsa. Erik Meijer, also working at the University
+of Utrecht, invited me for a lecture, as such introducing me to Doaitse. Apart from being an outstanding computer
+scientist, Doaitse was the best people manager I have ever worked for. Erik does not need any introduction. He became
+a living legend. Also Graham Hutton worked at the University of Utrecht when I was working there. I was in good company.
+
+The second paper was written together with Erik Meijer and was presented at a conference organized by the Glasgow
+University, the center of Functional Programming in the UK (Philip Wadler and Simon Peyton Jones worked there).
+
+The third paper was written together with Doaitse Swierstra. It turned out to be a motivation for two type
+constructor classes,
+[arrows](https://link.springer.com/chapter/10.1007/11546382_2) and
+[applicatives](https://www.researchgate.net/publication/215446169_Applicative_Programming_with_Effects),
+based upon mathematical foundations: Arrow based libraries are pointfree effectful functional programming libraries.
+Applicative based libraries are pointful effectful functional programming libraries. The relationship between them was
+explored in
+[Arrows and applicatives](https://homepages.inf.ed.ac.uk/wadler/papers/arrows-and-idioms/arrows-and-idioms.pdf)
+
+The fourth paper was based on
+[Monad transformers and modular interpreters](https://dl.acm.org/doi/pdf/10.1145/199448.199528).
+I added catamorphisms and subtypes to make interpreter alternatives reusable. The paper has never been published.
+Anyway, somehow, surprisingly, the paper turned out to be available online and it has been cited several times.
+
+All this brings me to the progressive insight that motivates me to do this Lean `PSBP` project.
+
+What are the most appropriate mathematical foundations and corresponding type classes for effectful functional
+programming? The more powerful they are the less implementation flexibility they have. For example monadic parsers
+can parse context sensitive grammars, while applicative parsers cannot parse context sensitive grammars, but,
+applicative parsers allow for more flexible error handling than monadic parsers.
+
+Programming is also about elegance and programming libraries are also about ease of use. I.m.h.o. pointfree programming
+is more elegant than pointful programming and pointfree programming libraries are easier of use than pointful
+programming libraries.
+
+Of course this is a matter of taste, but let me motivate my taste ... .
+
+The `Applicative` specification and the `Monad` specification specify computation capabilities. Think of computations as
+effectful expressions. They are operational artifacts. They do not really have a meaning in the mathematical sense and
+cannot be given a meaningful name. How, for example, would you name expression `x * x` in `λ x => x * x` ?
+Just like expressions are evaluated to yield a value, computations, by somehow executing them, yield a value, but,
+somehow executing computations may also perform side effects along the way. The "somehow" in the previous sentence is
+important, because it depends on the materialization corresponding to instances of the type constructor classes in
+terms of whose members the computations (recall, more precisely, computation specificatons) have been written.
+
+The program specification of this document is similar to, but more powerful than, the arrow specification. Think of
+programs as arrows with choice.
+
+The program specification of this document specifies, not surprisingly, program capabilities. Think of programs as
+effectful functions. They are denotational artifacts. They do have a meaning in the mathematical sense and can be given
+a meaningful name. For example `λ x => x * x` can be given a the meaningful name `square`. Of course functions and
+programs can also be looked at as operational artifacts. Just like functions, programs, by somehow running
+them, transform an initial value to a final value, but, somehow running them may perform side effects along the way. The
+"somehow" in the previous sentence is important, because it depends on the materialization corresponding to instances of
+the type constructor classes in terms of whose members the programs (recall, more precisely, program specificaton) have
+been written.
+
+By the way, a value can be a basic-value or a composite-value, repesented as a (nested) tuple. As such
+values are also components of a component system.
+
+Why going for pointfree programs instead of pointful applicatives or pointful monads?
+I.m.h.o. it is more natural to think denotationally, about "what", than to think operationally, about "how".
+
+Let's try to illustrate this with some `Lean` code.
+
+The computing related type class `Bind` has a member
+
+```
+bind :
+  {α β : Type} →
+  computation α → (α → computation β) → computation β
+```
+
+with an associativity law (`>>=` is infix notation for `bind`)
+
+```
+bind_assoc
+  (cα : computation α)
+  (αfcβ : α → computation β)
+  (βfcγ : β → computation γ) :
+    cα >>= αfcβ >>= βfcγ = cα >>=
+      λ α => αfcβ α >>= βfcγ
+```
+
+The programming related type class `Sequential` has a member
+
+```
+andThen
+  {α β γ : Type} :
+  program α β → program β γ → program α γ
+```
+
+with an associativity law (`>=>` is infix notation for `andThen`)
+
+```
+andThen_assoc
+  (αpβ : program α β)
+  (βpγ : program β γ)
+  (γpδ : program γ δ) :
+  (αpβ >=> βpγ) >=> γpδ =
+    αpβ >=> (βpγ >=> γpδ)
+```
+
+Let's first consider syntax.
+
+I can more easily remember the definition of `andThen_assoc` than the definition of `bind_assoc`.
+
+What about you?
+
+Let's next consider semantics.
+
+I can more easily explain `andThen` and `andThen_assoc` than `bind` and `bind_assoc`. I'll give it a try.
+
+What about you? Give it a try.
+
+Let's first deal with `Sequential`.
+
+I think of a function as transforming an initial value yielding a final value (transforming an argument to a result).
+
+Likewise, I think of a program as transforming an initial value yielding a final value (transforming an argument to a
+result (potentially performing side effects along the way)).
+
+Let's ignore side effects for now (you may wish to explain what happens with them).
+
+`andThen` can be explained as:
+
+transforming an initial value of type `α`, using a program of type `program α β`, yielding an intermediate value of type
+`β`, and then transforming that intermediate value, using a program of type `program β γ`, yielding a final value of
+type `γ`.
+
+`andThen_assoc` can be explained as:
+
+first transforming an initial value of type `α`, using `αpβ >=> βpγ`, yielding an intermediate value of type `γ`, and
+then transforming that intermediate value, using `γpδ`, yields the same final value as first transforming the initia
+value of type `α`, using `αpβ`, to an intermediate value of type `β`, and then transforming that intermediate value,
+using `βpγ >=> γpδ`.
+
+Let's second deal with `Bind`.
+
+I think of a evaluating an expression as yielding a value.
+
+Likewise, I think of a executing a computation as yielding a value (potentially performing side effects along the way).
+
+Let's ignore side effects for now  (you may wish to explain what happens with them).
+
+`bind` can be explained as:
+
+executing an inner computation of type `computation α` yielding an intermediate value of type `α`, and then binding that
+intermediate value to an outer computation valued function of type `α → computation β`, yields an outer computation of
+type `computation β` (that when executing it yields a value of type `β`)
+
+or
+
+executing an inner computation of type `computation α` yielding an intermediate value of type `α`, and then transforming
+that intermediate value using an outer computation valued function of type `α → computation β`, yields an outer
+computation value of type `computation β` (that when executing it yields a value of type `β`)
+
+`bind_assoc` can be explained as:
+
+executing an inner computation of `cα` yielding a first intermediate value, and then transforming that intermediate
+value using an intermediate computation valued function `αfcβ`, yielding an intermediate computation value that, when
+executing it, yields a second intermediate value, and then transforming that intermediate value using a final
+computation valued function `βfcγ` yields the same final outer computation value as executing the inner computation of
+`cα` yielding a first intermediate value, and then transforming that intermediate value using the computation valued
+function that first transforms that first intermediate value using the intermediate computation valued function `αfcβ`,
+yielding an intermediate computation value that, when executing it, yields a second intermediate value, and then
+transforming that intermediate value using a final computation valued function `βfcγ`.
+
+As far as components of a component system is concerned, I also like programs more than computations.
+
+Let's have a closer look at the associativity law code fragments
+
+```
+(αpβ >=> βpγ) >=> γpδ =
+  αpβ >=> (βpγ >=> γpδ)
+```
+
+and
+
+```
+cα >>= αfcβ >>= βfcγ =
+  cα >>= λ α => αfcβ α >>= βfcγ
+```
+
+Programs are closed components, while computations are open components. Computation `cα` needs to be opened to access
+the value `α` yielded by executing it, so that it can be transformed using computation valued function `αfcβ`.
+Programming with computations is pointful programming.
+
+Programs do not need to be opened. Programming with programs is pointfree programming. Think of using them as playing
+with Lego ariifacts.
+
+I.m.h.o, it is a more elegant and easier to program pointfree than to program pointful. Likewise, i.m.h.o., it is more
+elegant and easier to reason in terms of pointfree laws than to reason in terms of pointful laws. Of course, this is a
+matter of taste. Nevertheless hope to convince you that pointfree is more better than pointful.
+
+It is possible, and sometimes more elegant, use programs positionally. Positional programming is similar to pointful
+programming. It is is useful for writing sequential recipe-like programs, where, starting from an initial value
+(often a composite-value), intermediate values (mostly basic-values) are created, and, together with the initial value,
+as a compositional value are passed to the next step of the recipe-like program, until a final value is yielded. The
+initial value and intermediate values are accessed positionally. The creation of the intermediate values can involve
+general programs. A sequential recipe-like program glues programs together, similar to an operating system scripting
+language gluing operating system executables together.
+
+# The `PSBP` library type classes
+
+The `PSBP` library type classes are binary type constructor classes, but we also simply call them type classes.
 
 ## `class Functional`
 
-Functions can, somehow, be used as programs. Well, functions are what pure functional programming is all about.
-Functions that are used as programs are effectfree. We can define functions as programs in a formal way by defining a
-type class. This is what we do with the `Functional` type class.
+Functions can, somehow, be used as programs. Functions that are used as programs are effectfree. We can define functions
+as programs in a formal way by defining a type class. This is what we do with the `Functional` type class.
 
-```savedLean
+```lean
 class Functional
     (program : Type → Type → Type) where
   asProgram {α β : Type} :
@@ -76,14 +407,12 @@ class Functional
 export Functional (asProgram)
 ```
 
-A program, just like a function, transforms an initial value, its argument, to a final one, its result.
-
 ## `class Functorial`
 
 Functions can act upon programs. They act in an effectfree way. We can define functions acting upon programs in a formal
 way by defining a type class. This is what we do with the `Functorial` type class.
 
-```savedLean
+```lean
 class Functorial
     (program : Type → Type → Type) where
   andThenF {α β γ : Type} :
@@ -96,37 +425,15 @@ infixl:50 " >-> " => andThenF
 
 `andThenF` also has infix notation `>->`.
 
-We have used, and will continue to use, suffux `F` to distinguish functions from corresponding functions as programs.
-
-## `class Creational`
-
-Programs can be combined to produce product values. Their effects are accumulated from left to right. We can define
-programs that produce product values in a formal way by defining a type class. This is what we do with the `Creational`
-type class.
-
-```savedLean
-class Creational
-    (program : Type → Type → Type) where
-  product {α β γ : Type} :
-    program α β → program α γ → program α (β × γ)
-
-export Creational (product)
-
-infixl:60 " &&& " => product
-```
-
-`product` also has infix notation `&&&`.
-
-
 ## `class Sequential`
 
-Programs can be sequentially composed. Their effects are accumulated from left to right. Sequentially composing programs
-can be seen as a second program acting upon a first program. The difference with `Functorial` is that the second program
-may be effectful. Effects of the second program can depend on the final value of the first program. We can define
-programs that are sequentially composed in a formal way by defining a type class. This is what we do with the
+Programs can be sequentially combined. Sequentially combining programs can be seen as a second program acting upon a
+first program. The difference with `Functorial` is that the second program may be effectful. Their effects are
+accumulated from left to right. Effects of the second program can depend on the final value of the first program. We can
+define programs that are sequentially combined in a formal way by defining a type class. This is what we do with the
 `Sequential` type class.
 
-```savedLean
+```lean
 class Sequential
     (program : Type → Type → Type) where
   andThen {α β γ : Type} :
@@ -139,11 +446,32 @@ infixl:50 " >=> " => andThen
 
 `andThen` also has infix notation `>=>`.
 
+## `class Creational`
+
+Programs can be combined to create product values. Their effects are accumulated from left to right. We can define
+programs that produce product values in a formal way by defining a type class. This is what we do with the `Creational`
+type class.
+
+```lean
+class Creational
+    (program : Type → Type → Type) where
+  product {α β γ : Type} :
+    program α β → program α γ → program α (β × γ)
+
+export Creational (product)
+
+infixl:60 " &&& " => product
+```
+
+`product` also has infix notation `&&&`.
+
 ## `class Conditional`
 
-Programs can be combined to consume sum values. Only the left one or right one is used.
+Programs can be combined to consume sum values. Only the left one and its effects or right one and its effects is used.
+We can define programs that consume sum values in a formal way by defining a type class. This is what we do with the
+`Conditional` type class.
 
-```savedLean
+```lean
 class Conditional
     (program : Type → Type → Type) where
   sum {α β γ : Type} :
@@ -156,33 +484,33 @@ infixl:55 " ||| " => sum
 
 `sum` also has infix notation `|||`.
 
+## Writing programs
 
-## Capability combinations
+Programs are written in terms of members of type classes like the ones defined so far. The type class members are not
+defined, they are declared. Type classes are specifications. The programs written in terms of their members are program
+specifications, but, by abuse of language we call them programs.
 
-The idea behind writing programs in terms of type classes like the ones defined so far is to use exactly those
-capabilities that are necessary to write the programs. Some combinations of type classes are more expressive than
-other combinations. This implies that what you can do with them is more than what you can do the less expressive ones.
-But this comes with a price. They are less flexible as far as implementation and corresponding materialization is
-concerned than the less expressive ones.
+It is challenging to limit the expressiveness of the type class combinations in terms of whose members programs are
+written. More specification expressivenes implies less implementation flexibility.
 
-## Programs and program combinators defined in terms of the basic ones
+# `fibonacci` and `factorial`
 
-### `def identity`
+It turns out that we ready now for defining `fibonacci` and `factorial`.
 
-Below is a simple, but extremely useful function as a program, the `identity` program.
+The `identity` program is a simple, but extremely useful function as a program.
 
-```savedLean
+```lean
 def identity
     [Functional program] :
   program α α :=
     asProgram id
 ```
 
-### `def let_`
+## `def let_`
 
 Using the `let_` combinator an intermediate value can be constructed that is available for later use.
 
-```savedLean
+```lean
 def let_
     [Functional program]
     [Sequential program]
@@ -193,25 +521,15 @@ def let_
  def in_ : α → α := id
 ```
 
-The `p` in `αpβ` and `αaβpγ` stands for "program", and that the `a` in `αaβpγ` stands for "and". Think of `let_` as a
-library level keyword. `in_` is also a library level keyword that, depending on your taste, may make programs more
-readable.
+Think of `let_` as a library level keyword. `in_` is also a library level keyword that, depending on your taste, may
+make programs more readable.
 
-### `def if_`
+## `def if_`
 
 Using the `if_` combinator conditional boolean logic can be expressed. A helper function and corresponding program is
 needed to define it.
 
-```savedLean
-def trueToLeftFalseToRightF : α × Bool → α ⊕ α
-  | ⟨α, true⟩ => .inl α
-  | ⟨α, false⟩ => .inr α
-
-def trueToLeftFalseToRight
-    [Functional program] :
-  program (α × Bool) (α ⊕ α) :=
-    asProgram trueToLeftFalseToRightF
-
+```lean
 def if_
     [Functional program]
     [Sequential program]
@@ -224,21 +542,18 @@ def if_
     λ αpb t_apβ f_apβ =>
       let_ αpb $
         in_ $
-          trueToLeftFalseToRight >=>
+          asProgram (
+            λ αab => match αab with
+              | ⟨α, true⟩ => .inl α
+              | ⟨α, false⟩ => .inr α
+          ) >=>
           t_apβ ||| f_apβ
 
-def else_ {α} : α → α := id
+def else_ : α → α := id
 ```
-
-The `b` in `αpb` stands for `Bool`.
-
-# `fibonacci` and `factorial`
-
-It turns out that we ready now for defining `fibonacci` and `factorial`.
-
 For readability and reusability reasons it is useful to first define some primitive functions
 
-```savedLean
+```lean
 def isZeroF: Nat → Bool :=
   λ n => n == 0
 
@@ -263,7 +578,7 @@ def multiplyF : Nat × Nat → Nat :=
 
 and corresponding primitive programs
 
-```savedLean
+```lean
 def isZero
     [Functional program] :
   program Nat Bool :=
@@ -302,7 +617,7 @@ def multiply
 
 Program `fibonacci` is defined as follows
 
-```savedLean
+```lean
 unsafe def fibonacci
     [Functional program]
     [Creational program]
@@ -320,7 +635,7 @@ unsafe def fibonacci
 
 Program `factorial` is defined as follows
 
-```savedLean
+```lean
 unsafe def factorial
     [Functional program]
     [Creational program]
@@ -346,7 +661,7 @@ also a (special kind of) description.
 You may wonder why neither `fibonacci` nor `factorial` use `Functorial`. A `Functorial` instance can be defined in terms
 of `Function` and `Sequential`.
 
-```savedLean
+```lean
 instance
     [Functional program]
     [Sequential program] :
@@ -356,15 +671,13 @@ instance
       λ αpβ => λ βfγ => αpβ >=> asProgram βfγ
 ```
 
-The `f` in `βfγ` stands for "function".
-
 So why introducing `Functorial` in the first place? Well, the combination of `Functorial` with `Functional`, and
 `Creational` is sufficiently expressive to write interesting programs that are more flexible as far as implementation
 and corresponding materialization is concerned than the ones using `Sequential`.
 
 Below are two programs, `twiceMinusOne01` and `twiceMinusOne02`.
 
-```savedLean
+```lean
 def twiceMinusOne01
     [Functional program]
     [Functorial program]
@@ -391,12 +704,224 @@ implementation and corresponding materialization flexibility when dealing with e
 example is more flexible error handling when processing a submitted web form and even error correction when parsing a
 document.
 
+# Laws
+
+## `def identity`
+
+## `class LawfulFunctional`
+
+`Functional` comes with laws.
+
+```lean
+class LawfulFunctional (program : Type → Type → Type)
+    [Functional program]
+    [Sequential program] : Prop where
+  functional_identity :
+    (asProgram id : program α α) =
+      identity
+  functional_sequential
+      (αfβ : α → β)
+      (βfγ : β → γ) :
+    (asProgram αfβ >=> asProgram βfγ : program α γ) =
+      asProgram (βfγ ∘ αfβ)
+```
+
+The `functional_identity` law relates function identity and program identity, and is `True` per definition.
+
+The `functional_sequential` law relates function sequential combination and program sequential combination.
+
+## `class LawfulFunctorial`
+
+`Functorial` comes with laws.
+
+```lean
+class LawfulFunctorial (program : Type → Type → Type)
+    [Functorial program] : Prop where
+  functorial_identity
+    (αpβ : program α β) :
+    (αpβ >-> id : program α β) =
+      αpβ
+  functorial_sequential
+      (αpβ : program α β)
+      (βfγ : β → γ)
+      (γfδ : γ → δ) :
+    ((αpβ >-> βfγ) >-> γfδ) =
+      (αpβ >-> (γfδ ∘ βfγ))
+```
+
+The `functorial_identity` law states that the identity function action on a program leaves the program intact.
+
+The `functorial_sequential` law relates function sequential combination and function action sequential combination.
+
+## `class LawfulSequential`
+
+`Functorial` comes with laws.
+
+```lean
+class LawfulSequential (program : Type → Type → Type)
+    [Functional program]
+    [Sequential program] : Prop where
+  sequential_right_identity
+      (αpβ : program α β) :
+    (αpβ >=> identity : program α β) =
+      αpβ
+  sequential_left_identity
+      (αpβ : program α β) :
+    (identity >=> αpβ : program α β) =
+      αpβ
+  sequential_associativity
+      (αpβ : program α β)
+      (βpγ : program β γ)
+      (γpδ : program γ δ) :
+    ((αpβ >=> βpγ) >=> γpδ) =
+      (αpβ >=> (βpγ >=> γpδ))
+```
+
+The `sequential_right_identity` law states that the sequential combination of a program with the identity program at
+right leaves the program intact.
+
+The `sequential_left_identity` law states that the sequential combination of a program with the identity program at
+left leaves the program intact.
+
+The `sequential_associativity` law states that the sequential combination of programs is associative.
+
+## `class LawfulCreational`
+
+`applyAtFirst`, `applyAtSecond`, `onlyFirst` and `assoc` are used in the `Creational` laws below.
+
+```lean
+def applyAtFirst
+    [Functional program] :
+  (α → β) → program (α × γ) (β × γ) :=
+    λ αfβ => asProgram λ (α, γ) => (αfβ α, γ)
+```
+
+```lean
+def applyAtSecond
+    [Functional program] :
+  (β → γ) → program (α × β) (α × γ) :=
+    λ βfγ => asProgram λ (α, β) => (α, βfγ β)
+```
+
+and, let
+
+```lean
+def first
+    [Functional program] :
+  program (α × β) α :=
+    asProgram λ (α, _) => α
+```
+
+and
+
+```lean
+def second
+    [Functional program] :
+  program (α × β) β :=
+    asProgram λ (_, β) => β
+```
+
+in
+
+```lean
+def onlyFirst
+    [Functional program]
+    [Creational program]
+    [Sequential program] :
+  program α β → program (α × γ) (β × γ) :=
+    λ αpβ => (first >=> αpβ) &&& second
+```
+
+and
+
+```lean
+def assoc
+    [Functional program] :
+  program ((α × β) × γ) (α × (β × γ)) :=
+    asProgram (λ ((a, b), c) => (a, (b, c)))
+```
+
+`Creational` comes with laws.
+
+```lean
+class LawfulCreational (program : Type → Type → Type)
+    [Functional program]
+    [Sequential program]
+    [Creational program] : Prop where
+  creational_onlyFirst_asProgram
+      (αfβ : α → β) :
+    (onlyFirst (asProgram αfβ)
+      : program (α × γ) (β × γ)) =
+      applyAtFirst αfβ
+  creational_onlyFirst_sequential
+      (αpβ : program α β)
+      (βpγ : program β γ) :
+    (onlyFirst (αpβ >=> βpγ) :
+      program (α × δ) (γ × δ)) =
+      (onlyFirst αpβ >=> onlyFirst βpγ)
+  creational_onlyFirst_first
+      (αpβ : program α β) :
+    (onlyFirst αpβ >=> (first : program (β × γ) β)
+      : program (α × γ) β) =
+      ((first : program (α × γ) α) >=> αpβ)
+  creational_onlyFirst_applyAtSecond
+      (αpβ : program α β)
+      (γfδ : γ → δ) :
+    (onlyFirst αpβ >=> applyAtSecond γfδ
+      : program (α × γ) (β × δ)) =
+      (applyAtSecond γfδ >=> onlyFirst αpβ)
+  creational_onlyFirst_assoc
+      (αpβ : program α β) :
+    (onlyFirst (onlyFirst αpβ) >=> assoc
+      : program ((α × γ) × δ) (β × (γ × δ))) =
+      (assoc >=> onlyFirst αpβ)
+```
+
+## `class LawfulConditional`
+
+`left` and `right` are used in the `Conditional` laws below.
+
+```lean
+def left
+    [Functional program] :
+  program γ (γ ⊕ β) :=
+    asProgram .inl
+```
+
+and
+
+```lean
+def right
+    [Functional program] :
+  program β (γ ⊕ β) :=
+    asProgram .inr
+```
+
+`Conditional` comes with laws.
+
+```lean
+class LawfulConditional (program : Type → Type → Type)
+    [Functional program]
+    [Sequential program]
+    [Conditional program] : Prop where
+  conditional_left
+      (γpα : program γ α)
+      (βpα : program β α) :
+    (left >=> γpα ||| βpα) =
+      γpα
+  conditional_right
+      (γpα : program γ α)
+      (βpα : program β α) :
+    (right >=> γpα ||| βpα) =
+      βpα
+```
+
 # Computation Valued Functions
 
 Using computation valued functions is a generic way to implement the program related type classes in terms of the
 computation related type classes
 
-```savedLean
+```lean
 structure FromComputationValuedFunction
     (computation : (Type → Type)) (α β : Type) where
   toComputationValuedFunction : α → computation β
@@ -417,7 +942,8 @@ instance [Applicative computation] :
     Creational
       (FromComputationValuedFunction computation) where
   product := λ ⟨αfcβ⟩ ⟨αfcγ⟩ =>
-    ⟨λ α => pure .mk <*> αfcβ α <*> αfcγ α⟩
+    -- ⟨λ α => pure .mk <*> αfcβ α <*> αfcγ α⟩
+    ⟨λ α => .mk <$> αfcβ α <*> αfcγ α⟩
 
 instance [Monad computation] :
     Sequential
@@ -439,12 +965,485 @@ instance :
   sum := λ ⟨γfγα⟩ ⟨βfγα⟩ => ⟨foldSum γfγα βfγα⟩
 ```
 
-The the `c` in `αfcβ` stands for "computation".
-
 A word of warning, The code above sometimes uses `⟨` and `⟩`, different from `(` and `)`, to asemble and disassemble
 `structure`'s like `FromComputationValuedFunction`.
 
-# `ActiveProgram`
+# Theorems
+
+The laws of the various type classes need to be proved for the various instances. First we prove them and next we let
+`Lean` prove them for us.
+
+## `Functional` theorems
+
+Theorem `functional_identity` below is proved by definition using `by calc` and
+`rfl`.
+
+```lean
+@[simp] theorem functional_identity
+  {α : Type}
+    [Applicative computation] :
+    (identity :
+      FromComputationValuedFunction computation α α)
+      = asProgram id := by
+  calc
+    identity
+        = asProgram id
+          := rfl
+```
+Theorem `functional_sequential'` also uses `congrArg` and `funext`.
+
+Theorem `functional_sequential'` uses the `pure_bind` law of `LawfulMonad`.
+
+```lean
+theorem functional_sequential'
+  {α β γ : Type}
+    [Monad computation]
+    [LawfulMonad computation]
+  (αfβ : α → β)
+  (βfγ : β → γ) :
+    (asProgram αfβ >=> asProgram βfγ :
+      FromComputationValuedFunction computation α γ)
+      = asProgram (βfγ ∘ αfβ) := by
+  calc
+    (asProgram αfβ >=> asProgram βfγ :
+      FromComputationValuedFunction computation α γ)
+        = (⟨λ α => pure $ αfβ α⟩ >=> ⟨λ β => pure $ βfγ β⟩)
+          := rfl
+    _   = ⟨λ α => (pure $ αfβ α) >>= λ β => pure $ βfγ β⟩
+          := rfl
+    _   = ⟨λ α => pure $ βfγ (αfβ α)⟩
+          := congrArg
+               FromComputationValuedFunction.mk
+               (funext λ α =>
+                 pure_bind (αfβ α) (λ β => pure $ βfγ β))
+    _   = ⟨λ α => pure $ (βfγ ∘ αfβ) α⟩
+          := rfl
+    _   = asProgram (βfγ ∘ αfβ)
+          := rfl
+```
+
+Theorem `functional_sequential` uses `by simp` to let `Lean` do the heavy lifting
+
+```lean
+@[simp] theorem functional_sequential
+  {α β γ : Type}
+    [Monad computation]
+    [LawfulMonad computation]
+  (αfβ : α → β)
+  (βfγ : β → γ) :
+    (asProgram αfβ >=> asProgram βfγ :
+      FromComputationValuedFunction computation α γ)
+      = asProgram (βfγ ∘ αfβ) := by
+  simp[asProgram, andThen]
+```
+
+Note that `functional_sequential` is not annotated by `@[simp]` so that `functional_sequential'` cannot use it. As a
+consequence it is necessary to tell `Lean` to unfold everything in order for it to see the real definitions involved.
+
+## `Functorial` theorems
+
+Theorem `functorial_identity'` the `id_map` law of `LawfulFunctor`.
+
+```lean
+theorem functorial_identity'
+  {α β : Type}
+    [Functor computation]
+    [LawfulFunctor computation]
+  (αpβ : FromComputationValuedFunction computation α β) :
+    (αpβ >-> id :
+      FromComputationValuedFunction computation α β)
+      = αpβ := by
+  let αfcβ := αpβ.toComputationValuedFunction
+  calc
+    (αpβ >-> id)
+        = ⟨λ α => id <$> αfcβ α⟩
+          := rfl
+    _   = ⟨λ α => αfcβ α ⟩
+          := congrArg
+               FromComputationValuedFunction.mk
+               (funext λ α => id_map (αfcβ α))
+    _   = ⟨αfcβ⟩
+          := rfl
+```
+
+Theorem `functorial_identity` uses `simp` to let `Lean` do the heavy lifting
+
+```lean
+@[simp] theorem functorial_identity
+  {α β : Type}
+    [Functor computation]
+    [LawfulFunctor computation]
+  (αpβ : FromComputationValuedFunction computation α β) :
+    (αpβ >-> id :
+      FromComputationValuedFunction computation α β)
+      = αpβ := by
+    simp[andThenF]
+```
+
+Theorem `functorial_sequential'` uses the `comp_map` law of `LawfulFunctor`.
+
+```lean
+theorem functorial_sequential'
+  {α β γ δ : Type}
+    [Functor computation]
+    [LawfulFunctor computation]
+  (αpβ : FromComputationValuedFunction computation α β)
+  (βfγ : β → γ)
+  (γfδ : γ → δ) :
+    ((αpβ >-> βfγ) >-> γfδ :
+      FromComputationValuedFunction computation α δ)
+      = (αpβ >-> (γfδ ∘ βfγ)) := by
+  let αfcβ := αpβ.toComputationValuedFunction
+  calc
+    ((αpβ >-> βfγ) >-> γfδ)
+        = (⟨λ α => βfγ <$> αfcβ α⟩ >-> γfδ)
+          := rfl
+    _   = ⟨λ α => γfδ <$> (λ α => βfγ <$> αfcβ α) α⟩
+          := rfl
+    _   = ⟨λ α => γfδ <$> βfγ <$> αfcβ α⟩
+          := rfl
+    _   = ⟨λ α => (γfδ ∘ βfγ) <$> αfcβ α⟩
+          := congrArg
+               FromComputationValuedFunction.mk
+               (funext λ α =>
+                 Eq.symm (comp_map βfγ γfδ (αfcβ α)))
+    _   = (αpβ >-> (γfδ ∘ βfγ))
+          := rfl
+```
+
+Theorem `functorial_sequential` uses `simp` to let `Lean` do the heavy lifting
+
+```lean
+@[simp] theorem functorial_sequential
+    {α β γ δ : Type}
+    [Functor computation]
+    [LawfulFunctor computation]
+  (αpβ : FromComputationValuedFunction computation α β)
+  (βfγ : β → γ)
+  (γfδ : γ → δ) :
+    ((αpβ >-> βfγ) >-> γfδ :
+      FromComputationValuedFunction computation α δ)
+      = (αpβ >-> (γfδ ∘ βfγ)) := by simp[andThenF, comp_map]
+```
+
+## `Sequential` theorems
+
+Theorem `sequential_right_identity'` uses the `bind_pure_comp` law of `LawfulMonad` and the `comp_map` law of
+`LawfulFunctor`.
+
+```lean
+theorem sequential_right_identity'
+  {α β : Type}
+    [Monad computation]
+    [LawfulMonad computation]
+  (αpβ : FromComputationValuedFunction computation α β) :
+    (αpβ >=> asProgram id :
+      FromComputationValuedFunction computation α β)
+    = αpβ := by
+   let αfcβ := αpβ.toComputationValuedFunction
+   calc
+      (αpβ >=> asProgram id :
+          FromComputationValuedFunction computation α β)
+          = ⟨λ α => αfcβ α >>= λ β => pure (id β)⟩
+            := rfl
+      _   = ⟨λ α => id <$> αfcβ α⟩
+            := congrArg
+                 FromComputationValuedFunction.mk
+                 (funext λ α => bind_pure_comp id (αfcβ α))
+      _   = ⟨λ α => αfcβ α⟩
+            := congrArg
+                 FromComputationValuedFunction.mk
+                 (funext λ α => id_map (αfcβ α))
+      _   = αpβ
+            := rfl
+```
+
+Theorem `sequential_right_identity` uses `simp` to let `Lean` do the heavy lifting
+
+```lean
+@[simp] theorem sequential_right_identity
+  {α β : Type}
+    [Monad computation]
+    [LawfulMonad computation]
+  (αpβ : FromComputationValuedFunction computation α β) :
+    ((αpβ >=> asProgram id) :
+      FromComputationValuedFunction computation α β)
+      = αpβ := by simp[andThen]
+```
+
+Theorem `sequential_left_identity'` uses the `pure_bind` law of `LawfulMonad`.
+
+```lean
+@[simp] theorem sequential_left_identity'
+  {α β : Type}
+    [Monad computation]
+    [LawfulMonad computation]
+  (αpβ : FromComputationValuedFunction computation α β) :
+    (asProgram id >=> αpβ :
+      FromComputationValuedFunction computation α β)
+    = αpβ := by
+    let αfcβ := αpβ.toComputationValuedFunction
+    calc
+      (asProgram id >=> ⟨αfcβ⟩ :
+        FromComputationValuedFunction computation α β)
+          = ⟨λ α => pure α >>= αfcβ⟩
+            := rfl
+      _   = ⟨λ α => αfcβ α⟩
+            := congrArg
+                 FromComputationValuedFunction.mk
+                 (funext λ α => pure_bind α αfcβ)
+      _   = ⟨αfcβ⟩
+            := rfl
+```
+
+Theorem `sequential_left_identity` uses `simp` to let `Lean` do the heavy lifting
+
+```lean
+@[simp] theorem sequential_left_identity
+  {α β : Type}
+    [Monad computation]
+    [LawfulMonad computation]
+  (αpβ : FromComputationValuedFunction computation α β) :
+    (asProgram id >=> αpβ :
+      FromComputationValuedFunction computation α β)
+    = αpβ := by simp[andThen]
+```
+
+Theorem `sequential_associative'` uses the `pure_assoc` law of `LawfulMonad`.
+
+```lean
+@[simp] theorem sequential_associative'
+  {α β γ δ : Type}
+    [Monad computation]
+    [LawfulMonad computation]
+  (αpβ : FromComputationValuedFunction computation α β)
+  (βpγ : FromComputationValuedFunction computation β γ)
+  (γpδ : FromComputationValuedFunction computation γ δ) :
+    ((αpβ >=> βpγ) >=> γpδ :
+      FromComputationValuedFunction computation α δ) =
+      (αpβ >=> (βpγ >=> γpδ)) := by
+  let αfcβ : α → computation β :=
+    αpβ.toComputationValuedFunction
+  let βfcγ : β → computation γ :=
+    βpγ.toComputationValuedFunction
+  let γfcδ : γ → computation δ :=
+    γpδ.toComputationValuedFunction
+  let βfcδ : β → computation δ :=
+    λ β => βfcγ β >>= γfcδ
+  calc
+    ((αpβ >=> βpγ) >=> γpδ :
+      FromComputationValuedFunction computation α δ)
+        = (⟨λ α => αfcβ α >>= βfcγ⟩ >=> ⟨γfcδ⟩)
+          := rfl
+    _   = ⟨λ α => αfcβ α >>= βfcγ >>= γfcδ⟩
+          := rfl
+    _   = ⟨λ α => αfcβ α >>= (λ β => βfcγ β >>= γfcδ)⟩
+          := congrArg
+               FromComputationValuedFunction.mk
+               (funext λ α => bind_assoc (αfcβ α) βfcγ γfcδ)
+    _   = (⟨λ α => αfcβ α >>= βfcδ⟩ :
+            FromComputationValuedFunction computation α δ)
+          := rfl
+    _   = (αpβ >=> (βpγ >=> γpδ):
+            FromComputationValuedFunction computation α δ)
+          := rfl
+```
+
+Theorem `sequential_associative` uses `simp` to let `Lean` do the heavy lifting
+
+```lean
+@[simp] theorem sequential_associative
+  {α β γ δ : Type}
+    [Monad computation]
+    [LawfulMonad computation]
+  (αpβ : FromComputationValuedFunction computation α β)
+  (βpγ : FromComputationValuedFunction computation β γ)
+  (γpδ : FromComputationValuedFunction computation γ δ) :
+    ((αpβ >=> βpγ) >=> γpδ :
+      FromComputationValuedFunction computation α δ) =
+      (αpβ >=> (βpγ >=> γpδ)) := by simp[andThen]
+```
+
+# `Creational` theorems
+
+Theorem `creational_onlyFirst_asProgram'` uses the `pure_bind` law of `LawfulMonad` and the `map_pure` law of
+`LawfulApplicative`.
+
+```lean
+theorem creational_onlyFirst_asProgram'
+  {α β γ : Type}
+    [Monad computation]
+    [LawfulMonad computation]
+  (αfβ : α → β) :
+    (onlyFirst (asProgram αfβ) :
+      FromComputationValuedFunction
+        computation (α × γ) (β × γ)) =
+      (asProgram (λ (α, γ) => (αfβ α, γ))) := by
+  calc
+    (onlyFirst (asProgram αfβ))
+        = onlyFirst ⟨λ α => pure $ αfβ α⟩ :=
+        rfl
+    _   = ((first :
+           FromComputationValuedFunction
+             computation (α × γ) α) >=>
+            (⟨λ α => pure $ αfβ α⟩)) &&& second :=
+        rfl
+    _   = (((asProgram λ (α, _) => α) :
+            FromComputationValuedFunction
+              computation (α × γ) α) >=>
+              (⟨λ α => pure $ αfβ α⟩)) &&& second :=
+        rfl
+    _   = ((⟨λ (α, _) => pure α⟩ :
+            FromComputationValuedFunction
+              computation (α × γ) α) >=>
+              (⟨λ α => pure $ αfβ α⟩)) &&& second :=
+        rfl
+    _   = (⟨λ (α, _) => pure α >>= (λ α => pure $ αfβ α)⟩ :
+            FromComputationValuedFunction
+              computation (α × γ) β) &&& second :=
+        rfl
+    _   = (⟨(λ (α, _) => pure $ αfβ α)⟩ :
+            FromComputationValuedFunction
+              computation (α × γ) β) &&& second :=
+        congrArg
+          (λ (αfcβ : α → computation β) =>
+            ((⟨λ (α, _) => αfcβ α⟩ :
+            FromComputationValuedFunction
+              computation (α × γ) β) &&& second))
+          (funext (λ α =>
+            pure_bind α (λ α => pure $ αfβ α)))
+    _   = (⟨λ (α, _) => pure $ αfβ α⟩ :
+            FromComputationValuedFunction
+              computation (α × γ) β) &&& second :=
+        rfl
+    _   = (⟨λ (α, _) => pure $ αfβ α⟩ :
+            FromComputationValuedFunction
+              computation (α × γ) β) &&&
+              (asProgram (λ (_, γ) => γ) :
+                FromComputationValuedFunction
+                  computation (α × γ) γ) :=
+        rfl
+    _   = (⟨λ (α, _) => pure $ αfβ α⟩ :
+            FromComputationValuedFunction
+              computation (α × γ) β) &&&
+              (⟨λ (_, γ) => pure $ γ⟩ :
+                FromComputationValuedFunction
+                  computation (α × γ) γ) :=
+        rfl
+    _   = (⟨λ (α, γ) =>
+            (Prod.mk <$> (pure $ αfβ α)) <*> (pure $ γ)⟩ :
+             FromComputationValuedFunction
+               computation (α × γ) (β × γ)) :=
+        rfl
+    _   = (⟨λ (α, γ) =>
+            (pure $ Prod.mk (αfβ α)) <*> (pure $ γ)⟩ :
+             FromComputationValuedFunction
+             computation (α × γ) (β × γ)) :=
+        congrArg
+         (FromComputationValuedFunction.mk ∘
+           ((λ αfβaγ =>
+             λ (α, γ) => αfβaγ α <*> (pure $ γ)) :
+             (α → computation (γ → (β × γ))) →
+               ((α × γ) → computation (β × γ))))
+          (funext λ α => (map_pure (Prod.mk) (αfβ α)))
+    _   = (⟨λ (α, γ) => Prod.mk (αfβ α) <$> (pure $ γ)⟩) :=
+        congrArg
+         FromComputationValuedFunction.mk
+          (funext λ (α, γ) =>
+            (pure_seq (Prod.mk (αfβ α)) (pure $ γ)))
+    _   = (⟨λ (α, γ) => pure (Prod.mk (αfβ α) γ)⟩) :=
+        congrArg
+         FromComputationValuedFunction.mk
+          (funext λ (α, γ) =>
+            (map_pure (Prod.mk (αfβ α)) γ))
+    _   = (⟨λ (α, γ) => pure $ (αfβ α, γ)⟩) :=
+        rfl
+    _   = (asProgram (λ (α, γ) => (αfβ α, γ))) :=
+        rfl
+```
+
+Theorem `creational_onlyFirst_asProgram` uses `simp` to let `Lean` do the heavy lifting
+
+```lean
+@[simp] theorem creational_onlyFirst_asProgram
+  {α β γ : Type}
+    [Monad computation]
+    [LawfulMonad computation]
+  (αfβ : α → β) :
+    (onlyFirst (asProgram αfβ) :
+      FromComputationValuedFunction
+        computation (α × γ) (β × γ)) =
+      (asProgram (λ (α, γ) => (αfβ α, γ))) := by simp [
+        onlyFirst, asProgram, product, first, second
+        ]
+```
+
+By now you probably agree that `calc` based proofs can become tedious.
+
+In what follows, I will, mostly, only show the `simp` based proofs.
+
+```lean
+@[simp] theorem creational_onlyFirst_sequential
+  {α β γ : Type}
+    [Monad computation]
+    [LawfulMonad computation]
+  (αpβ : FromComputationValuedFunction computation α β)
+  (βpγ : FromComputationValuedFunction computation β γ) :
+    (onlyFirst (αpβ >=> βpγ) :
+      FromComputationValuedFunction
+        computation (α × δ) (γ × δ)) =
+      (onlyFirst αpβ >=> onlyFirst βpγ :
+        FromComputationValuedFunction
+          computation (α × δ) (γ × δ)) := by simp[
+            onlyFirst, andThen, asProgram, product, first,
+            second
+            ]
+```
+
+```lean
+@[simp] theorem creational_onlyFirst_first
+  {α β γ : Type}
+    [Monad computation]
+    [LawfulMonad computation]
+  (αpβ : FromComputationValuedFunction computation α β) :
+    (onlyFirst αpβ >=> first :
+      FromComputationValuedFunction computation (α × γ) β) =
+      (first >=> αpβ) := by simp[
+        onlyFirst, andThen, asProgram, product, first,
+        second
+        ]
+```
+
+```lean
+@[simp] theorem creational_onlyFirst_applyAtSecond
+  {α β γ δ : Type}
+    [Monad computation]
+    [LawfulMonad computation]
+  (αpβ : FromComputationValuedFunction computation α β)
+  (γfδ : γ → δ) :
+    (onlyFirst αpβ >=> applyAtSecond γfδ) =
+      (applyAtSecond γfδ >=> onlyFirst αpβ) := by simp[
+        onlyFirst, andThen, applyAtSecond, asProgram,
+        product, first, second
+        ]
+```
+
+```lean
+@[simp] theorem creational_onlyFirst_assoc
+  {α β γ δ : Type}
+    [Monad computation]
+    [LawfulMonad computation]
+  (αpβ : FromComputationValuedFunction computation α β) :
+    (onlyFirst (onlyFirst αpβ) >=> assoc :
+      FromComputationValuedFunction
+        computation ((α × γ) × δ) (β × (γ × δ))) =
+      (assoc >=> onlyFirst αpβ) := by simp[
+        onlyFirst, andThen, asProgram, product, first,
+        second, assoc
+        ]
+```
+
+## `ActiveProgram`
 
 There is not a lot of work to be done for active implementations. The `Functor`, `Applicative` and `Monad`
 implementations of `Id` can be used.
@@ -761,7 +1760,7 @@ def positionOneAndTwo
 -- ...
 ```
 
-`positionOne` and `positionTwo` are single-value positions. `positionOneAndTwo` is a multi-value position.
+`positionOne` and `positionTwo` are basic-value positions. `positionOneAndTwo` is a multi-value position.
 
 ## `positionalFactorialOfFibonacci` and `positionalSumOfFibonacciAndFactorial`
 
@@ -891,21 +1890,21 @@ The `σ` above stands for "state".
 
 Below is `modifyStateWith`, a useful programming with state capability.
 
-Let
+-- Let
 
-```savedLean
-def first
-    [Functional program] :
-  program (α × β) α :=
-    asProgram λ (α, _) => α
+-- ```savedLean
+-- def first
+--     [Functional program] :
+--   program (α × β) α :=
+--     asProgram λ (α, _) => α
 
-def second
-    [Functional program] :
-  program (α × β) β :=
-    asProgram  λ (_, β) => β
-```
+-- def second
+--     [Functional program] :
+--   program (α × β) β :=
+--     asProgram  λ (_, β) => β
+-- ```
 
-in (only `first` above is used)
+-- in (only `first` above is used)
 
 ```savedLean
 def modifyStateWith
